some work on replay

fr.inria.atlanmod.coqtl.coq/core/cached/Interpreter.v
@@ -7,6 +7,7 @@ Require Import Bool.
 Require Import core.Syntax.
 Require Import Arith.
 Require Import Semantics.
+Require Import List.
 
 Scheme Equality for list.
 
@@ -47,6 +48,7 @@ Section LazySemantics.
     | addElementToSource : SourceModelElement -> Stmt
     | deleteElementFromSource : SourceModelElement -> Stmt
     | addLinkToSource : SourceModelLink -> Stmt
+    | skip : Stmt
     .
 
     (* some helper of Model *)
@@ -68,26 +70,52 @@ Section LazySemantics.
        TODO: step : state -> state * output, this signature can show the output of the trace
      *)
     
-    Definition replay (s: Stmt) (st: State) : State * (option (list TargetModelElement)) :=
+    Definition strict_replay (s: Stmt) (st: State) : State * (option (list TargetModelElement)) :=
       match s with
+      | getRootFromTarget => (st, Some nil) (* accessing the function of the State typeclass *)
       | _ => (st, None)
       end.
-    
-    Definition replay_state (s: Stmt) (st: State) := (fst (replay s st)).
 
-    Definition replay_prog_state (st: State) (s: list Stmt) :=
-      fold_right (replay_state) st s.
+    Definition strict_replay_state (s: Stmt) (st: State) := (fst (strict_replay s st)).
+
+    Definition strict_replay_trace_state (st: State) (s: list Stmt) :=
+      fold_right strict_replay_state st s.
+
+    Definition replay_last_output (st: State) (s: list Stmt) :=
+      let endstate := fold_right (strict_replay_state) st (removelast s) in
+        (snd (strict_replay (last s skip) endstate)).
       
-    Definition strict_replay_trace (st: State) (tr: list Stmt) : list (option (list TargetModelElement)) :=
-      nil.
+    (* Theorem equivalence_strict_lazy:
+      forall (st: State) (trace: list Stmt),
+        list_beq (strict_replay_trace st trace) (lazy_replay_trace st trace).*)
 
-    Definition lazy_replay_trace (st: State) (tr: list Stmt) : list (option (list TargetModelElement)) :=
-      nil.
+    (*Theorem equivalence_strict_lazy:
+      forall (st: State) (trace: list Stmt),
+        beq (strict_replay_last_output st trace) (lazy_replay_last_output st trace).*)
+
+    Definition strict_replay' (s: Stmt) (st: State) : State :=
+      match s with
+      | getRootFromTarget => st (* accessing the function of the State typeclass *)
+      | _ => st
+      end.
+
+    Definition strict_replay_trace_state' (st: State) (s: list Stmt) :=
+      fold_right strict_replay' st s.
+
+    (*Definition replay_last_output' (st: State) (s: list Stmt) :=
+      let endstate := fold_right (strict_replay') st (removelast s) in
+        match (last s skip) with 
+        | getRootFromTarget => None
+        | _ => None
+        end.*)
+      
+    (* Theorem equivalence_strict_lazy:
+      forall (st: State) (trace: list Stmt),
+        list_beq (strict_replay_trace st trace) (lazy_replay_trace st trace).*)
 
     Theorem equivalence_strict_lazy:
       forall (st: State) (trace: list Stmt),
-        beq_list (strict_replay_prog st trace) (lazy_replay_prog st trace).
-        
+        beq (strict_replay_last_output st trace) (lazy_replay_last_output st trace).
 
     Fixpoint replay (tr: Transformation) (sm: SourceModel) (tm: TargetModel) (s: Stmt) : state :=
       match s with
@@ -96,9 +124,6 @@ Section LazySemantics.
       | addElementToSource se => conf tr (Model_addElementToSource sm se) (execute tr (Model_addElementToSource sm se)) skip
       | _ => error
       end.
-
-
-
 
     (* lazy semantics *)
 
@@ -125,7 +150,5 @@ Section LazySemantics.
 
     Definition trace :=
      replay tr sm (execute tr sm) exProg.
-
-
 
 End LazySemantics.
